\documentclass{jpmarticle}

\title{Crank--Nicolson for an SIR model}
\author{Jan Medlock}

\begin{document}

\maketitle

The model is
\begin{equation}
  \begin{split}
    \frac{\md S}{\md t} &= b(t) N - \beta I S - \mu S,
    \\
    \frac{\md I}{\md t} &= \beta I S - \gamma I - \mu I,
    \\
    \frac{\md R}{\md t} &= \gamma I - \mu R,
  \end{split}
\end{equation}
with birth rate
\begin{equation}
  b(t) = \mu \left[
    1 + \sigma \sqrt{2} \cos\left(2 \pi t\right)
  \right],
\end{equation}
and population size
\begin{equation}
  N(t) = S(t) + I(t) + R(t).
\end{equation}

The total population follows
\begin{equation}
  \begin{split}
    \frac{\md N}{\md t}
    &= b(t) N - \mu N
    \\
    &= \mu \sigma \sqrt{2} \cos\left(2 \pi t\right) N,
  \end{split}
\end{equation}
so that
\begin{equation}
  \log N(t) = \log N(0)
  + \frac{\mu \sigma}{\pi \sqrt{2}}
  \sin\left(2 \pi t\right),
\end{equation}
or
\begin{equation}
  N(t) = N(0) \exp\left[
    \frac{\mu \sigma}{\pi \sqrt{2}}
    \sin\left(2 \pi t\right)
  \right],
\end{equation}
i.e.~periodic with period $1$.

The model for log-transformed variables is
\begin{equation}
  \begin{split}
    \frac{\md S_{\log}}{\md t}
    &= b(t) \me^{\left(N_{\log} - S_{\log}\right)}
    - \beta \me^{I_{\log}}
    - \mu,
    \\
    \frac{\md I_{\log}}{\md t}
    &= \beta \me^{S_{\log}} - \gamma - \mu,
    \\
    \frac{\md R_{\log}}{\md t}
    &= \gamma \me^{\left(I_{\log} - R_{\log}\right)}
    - \mu,
  \end{split}
\end{equation}
with
\begin{equation}
  N_{\log} = \log\left(
    \me^{S_{\log}} + \me^{I_{\log}} + \me^{R_{\log}}
  \right).
\end{equation}

For the system of differential equations
\begin{equation}
  \begin{split}
    \frac{\md \vec{Y}}{\md t}
    &= \vec{f}\left(t, \vec{Y}\right),
    \\
    \vec{Y}(0) &= \vec{Y}^0,
  \end{split}
\end{equation}
and time step $\Delta t$, let $t^k = k \Delta t$ for
$k \in \{0, 1, \ldots, K - 1\}$ and
\begin{equation}
  \vec{Y}^k \approx \vec{Y}(t^k).
\end{equation}
The Crank--Nicolson scheme is
\begin{equation}
  \frac{\vec{Y}^k - \vec{Y}^{k - 1}}{\Delta t}
  = \frac{
    \vec{f}\left(t^k, \vec{Y}^k\right)
    + \vec{f}\left(t^{k - 1}, \vec{Y}^{k - 1}\right)
  }{2}
\end{equation}
for $k \in \{1, \ldots, K - 1\}$.
That is, to find $\vec{Y}^k$ such that
\begin{equation}
  \vec{Y}^k
  - \frac{\Delta t}{2}
  \vec{f}\left(t^k, \vec{Y}^k\right)
  - \vec{Y}^{k - 1}
  - \frac{\Delta t}{2}
  \vec{f}\left(t^{k - 1}, \vec{Y}^{k - 1}\right)
  = 0.
\end{equation}


\end{document}
